src/Init/Internal/MonadAttach.lean
@@ -9,27 +9,29 @@ prelude
 public import Init.System.IO
 import all Init.System.ST
 
-public class MonadAttach (m : Type u → Type v) [Monad m] where
+public class MonadAttach (m : Type u → Type v) where
   CanReturn : m α → α → Prop
   attach : (x : m α) → m (Subtype (CanReturn x))
-  map_val_attach : Subtype.val <$> attach x = x
 
 public class LawfulMonadAttach (m : Type u → Type v) [Monad m] [MonadAttach m] where
-  strongest {P : α → Prop} {x : m (Subtype P)} {a : α} :
-    MonadAttach.CanReturn (Subtype.val <$> x) a → P a
-  ump {P : α → Prop} {x : m (Subtype P)} :
-    (fun x => ⟨x.val, strongest x.property⟩) <$> MonadAttach.attach (Subtype.val <$> x) = x
+  map_val_attach {x : m α} : Subtype.val <$> MonadAttach.attach x = x
+  -- strongest {P : α → Prop} {x : m (Subtype P)} {a : α} :
+  --   MonadAttach.CanReturn (Subtype.val <$> x) a → P a
+  -- ump {P : α → Prop} {x : m (Subtype P)} :
+  --   (fun x => ⟨x.val, strongest x.property⟩) <$> MonadAttach.attach (Subtype.val <$> x) = x
 
 instance : MonadAttach IO where
   CanReturn x a := ∃ world world', x world = .ok a world'
   attach x := fun world => match h : x world with
     | .ok a world' => .ok ⟨a, world, world', h⟩ world'
     | .error e world' => .error e world'
+
+instance : LawfulMonadAttach IO where
   map_val_attach := by
     intro α x
     rw [funext_iff]
     intro world
-    simp only [Functor.map, EST.bind, Function.comp_apply]
+    simp only [Functor.map, EST.bind, Function.comp_apply, MonadAttach.attach]
     split <;> rename_i heq
     · split at heq
       · cases heq
