src/Init/Data/Iterators/Lemmas/Combinators/Monadic/FilterMap.lean
@@ -247,9 +247,8 @@ instance {α β γ : Type w} {m : Type w → Type w'} {n : Type w → Type w''} 
     have : it = IterM.mapWithPostcondition _ it.internalState.inner := by rfl
     generalize it.internalState.inner = it at *
     cases this
-    simp only [LawfulIteratorCollect.toArrayMapped_eq]
     simp only [IteratorCollect.toArrayMapped]
-    rw [LawfulIteratorCollect.toArrayMapped_eq]
+    simp only [LawfulIteratorCollect.toArrayMapped_eq]
     induction it using IterM.inductSteps with | step it ih_yield ih_skip
     rw [IterM.DefaultConsumers.toArrayMapped_eq_match_step]
     rw [IterM.DefaultConsumers.toArrayMapped_eq_match_step]
