src/Init/Data/Iterators/Lemmas/Consumers/Monadic/Loop.lean
@@ -18,53 +18,34 @@ theorem IterM.DefaultConsumers.forIn'_eq_match_step {α β : Type w} {m : Type w
     [Iterator α m β] {n : Type x → Type x'} [Monad n] [LawfulMonad n]
     {lift : ∀ γ δ, (γ → n δ) → m γ → n δ} {γ : Type x}
     {it : IterM (α := α) m β} {init : γ}
-    {P hP} {f : (b : β) → P b → (c : γ) → n (ForInStep γ)}
+    {P hP}
     (plausible_forInStep : β → γ → ForInStep γ → Prop)
-    (wf : IteratorLoop.WellFounded α m plausible_forInStep)
-    (f' : (b : β) → P b → (c : γ) → n (Subtype (plausible_forInStep b c)))
-    (hf : ∀ b h c, f b h c = Subtype.val <$> f' b h c) :
-    IterM.DefaultConsumers.forIn' lift γ it init P hP f =
+    {f : (b : β) → P b → (c : γ) → n (Subtype (plausible_forInStep b c))}
+    (wf : IteratorLoop.WellFounded α m plausible_forInStep) :
+    IterM.DefaultConsumers.forIn' lift γ plausible_forInStep it init P hP f =
       (lift _ _ · it.step) (fun s =>
           match s.inflate with
           | .yield it' out h => do
             match ← f out (hP _ <| .direct ⟨_, h⟩) init with
-            | .yield c =>
-              IterM.DefaultConsumers.forIn' lift _ it' c P
+            | ⟨.yield c, _⟩ =>
+              IterM.DefaultConsumers.forIn' lift _ plausible_forInStep it' c P
                 (fun _ h' => hP _ <| .indirect ⟨_, rfl, h⟩ h') f
-            | .done c => return c
+            | ⟨.done c, _⟩ => return c
           | .skip it' h =>
-            IterM.DefaultConsumers.forIn' lift _ it' init P
+            IterM.DefaultConsumers.forIn' lift _ plausible_forInStep it' init P
               (fun _ h' => hP _ <| .indirect ⟨_, rfl, h⟩ h') f
           | .done _ => return init) := by
   haveI : Nonempty γ := ⟨init⟩
-  rw [forIn', Internal.extrinsicFix₃_eq]
+  rw [forIn', Internal.extrinsicFixE₃_eq]
   · congr; ext step
-    cases step.inflate using PlausibleIterStep.casesOn <;> rfl
-  · refine ⟨?r, ?F', ?wf, ?h⟩
-    · exact InvImage (IteratorLoop.rel α m plausible_forInStep) (fun s => ⟨s.1, s.2.1⟩)
-    · exact fun it acc hP G => (
-      (lift _ _ · it.step) (fun s =>
-          match s.inflate with
-          | .yield it' out h => do
-            match ← f' out (hP _ <| .direct ⟨_, h⟩) acc with
-            | ⟨.yield c, h'⟩ =>
-              G it' c (fun _ h' => hP _ <| .indirect ⟨_, rfl, h⟩ h') (Or.inl ⟨out, h, h'⟩)
-            | ⟨.done c, _⟩ => return c
-          | .skip it' h =>
-            G it' acc (fun _ h' => hP _ <| .indirect ⟨_, rfl, h⟩ h') (Or.inr ⟨h, rfl⟩)
-          | .done _ => return acc))
-    · exact InvImage.wf _ wf
-    · intro it acc h G
-      simp only
-      congr 1; ext step
-      cases step.inflate using PlausibleIterStep.casesOn
-      · simp only [hf, map_eq_pure_bind, bind_assoc, pure_bind]
-        apply bind_congr; intro step
-        match step with
-        | ⟨.yield c, h⟩ => simp
-        | ⟨.done c, h⟩ => simp
-      · simp
-      · simp
+    cases step.inflate using PlausibleIterStep.casesOn
+    · simp only
+      apply bind_congr; intro step
+      split <;> simp [forIn']
+    · simp [forIn']
+    · simp
+  · apply InvImage.wf
+    exact wf
 
 theorem IterM.DefaultConsumers.forIn'_eq_wf {m : Type w → Type w'} {α : Type w} {β : Type w}
     [Iterator α m β]
@@ -74,42 +55,16 @@ theorem IterM.DefaultConsumers.forIn'_eq_wf {m : Type w → Type w'} {α : Type 
     (wf : IteratorLoop.WellFounded α m Pl)
     {it : IterM (α := α) m β} {init : γ}
     {P : β → Prop} {hP : ∀ b, it.IsPlausibleIndirectOutput b → P b}
-    (f : (b : β) → P b → (c : γ) → n (ForInStep γ))
-    (f' : (b : β) → P b → (c : γ) → n (Subtype (Pl b c)))
-    (hf : ∀ b h c, f b h c = Subtype.val <$> f' b h c) :
-    forIn' lift γ it init P hP f =
-      forIn'.wf lift γ Pl wf it init P hP f' := by
+    (f : (b : β) → P b → (c : γ) → n (Subtype (Pl b c))) :
+    forIn' lift γ Pl it init P hP f =
+      forIn'.wf lift γ Pl wf it init P hP f := by
   haveI : Nonempty γ := ⟨init⟩
-  rw [forIn', Internal.extrinsicFix₃_eq_wellFoundedFix]; rotate_left
-  · exact InvImage WellFoundedRelation.rel (fun x => IteratorLoop.WithWF.mk x.1 x.2.1 (hwf := wf))
-  · exact fun it acc hP G =>
-      (lift _ _ · it.step) fun s =>
-        match s.inflate with
-        | .yield it' out h => do
-          match ← f' out (hP _ <| .direct ⟨_, h⟩) acc with
-          | ⟨.yield c, h'⟩ =>
-            G it' c (fun _ h' => hP _ <| .indirect ⟨_, rfl, h⟩ h') (Or.inl ⟨_, ‹_›, ‹_›⟩)
-          | ⟨.done c, _⟩ => return c
-        | .skip it' h =>
-          G it' acc (fun _ h' => hP _ <| .indirect ⟨_, rfl, h⟩ h') (Or.inr ⟨‹_›, rfl⟩)
-        | .done _ => return acc
-  · exact InvImage.wf _ WellFoundedRelation.wf
-  · simp only
-    intro a c h G
-    congr 1; ext step
-    cases step.inflate using PlausibleIterStep.casesOn
-    · simp only
-      rw [hf, map_eq_pure_bind, bind_assoc]
-      apply bind_congr; intro forInStep
-      match forInStep with
-      | ⟨.yield c, h⟩ => simp
-      | ⟨.done c, h⟩ => simp
-    · simp
-    · simp
-  · fun_induction forIn'.wf lift γ Pl wf it init P hP f'
+  rw [forIn', Internal.extrinsicFixE₃_eq_wellFoundedFix]; rotate_left
+  · apply InvImage.wf
+    exact wf
+  · fun_induction forIn'.wf lift γ Pl wf it init P hP f
     rename_i ihy ihs
     rw [WellFounded.fix_eq]
-    simp only
     congr 1; ext step
     cases step.inflate using PlausibleIterStep.casesOn
     · apply bind_congr; intro forInStep
@@ -125,12 +80,10 @@ theorem IterM.DefaultConsumers.forIn'_eq_wf_of_finite {m : Type w → Type w'} {
     {lift : ∀ γ δ, (γ → n δ) → m γ → n δ} {γ : Type x}
     {it : IterM (α := α) m β} {init : γ}
     {P : β → Prop} {hP : ∀ b, it.IsPlausibleIndirectOutput b → P b}
-    (f : (b : β) → P b → (c : γ) → n (ForInStep γ)) :
-    forIn' lift γ it init P hP f =
-      forIn'.wf lift γ (fun _ _ _ => True) IteratorLoop.wellFounded_of_finite it init P hP
-        (fun b h c => (⟨·, trivial⟩) <$> f b h c) := by
+    (f : (b : β) → P b → (c : γ) → n (Subtype (fun _ => True))) :
+    forIn' lift γ (fun _ _ _ => True) it init P hP f =
+      forIn'.wf lift γ (fun _ _ _ => True) IteratorLoop.wellFounded_of_finite it init P hP f := by
   apply forIn'_eq_wf
-  simp
 
 theorem IterM.forIn'_eq {α β : Type w} {m : Type w → Type w'} [Iterator α m β] [Finite α m]
     {n : Type w → Type w''} [Monad m] [Monad n] [LawfulMonad n] [IteratorLoop α m n]
@@ -139,9 +92,9 @@ theorem IterM.forIn'_eq {α β : Type w} {m : Type w → Type w'} [Iterator α m
     {f : (b : β) → it.IsPlausibleIndirectOutput b → γ → n (ForInStep γ)} :
     letI : ForIn' n (IterM (α := α) m β) β _ := IterM.instForIn'
     ForIn'.forIn' (α := β) (m := n) it init f = IterM.DefaultConsumers.forIn' (n := n)
-        (fun _ _ f x => monadLift x >>= f) γ it init _ (fun _ => id) (f · · ·) := by
+        (fun _ _ f x => monadLift x >>= f) γ (fun _ _ _ => True) it init _ (fun _ => id) (return ⟨← f · · ·, trivial⟩) := by
   simp only [instForIn', ForIn'.forIn', IteratorLoop.finiteForIn']
-  have : (f · · ·) = (Subtype.val <$> (⟨·, trivial⟩) <$> f · · ·) := by simp
+  have : f = (Subtype.val <$> (⟨·, trivial⟩) <$> f · · ·) := by simp
   rw [this, hl.lawful (fun _ _ f x => monadLift x >>= f) (wf := IteratorLoop.wellFounded_of_finite)]
   simp [IteratorLoop.defaultImplementation]
 
@@ -151,7 +104,8 @@ theorem IterM.forIn_eq {α β : Type w} {m : Type w → Type w'} [Iterator α m 
     [MonadLiftT m n] [LawfulMonadLiftT m n] {γ : Type w} {it : IterM (α := α) m β} {init : γ}
     {f : β → γ → n (ForInStep γ)} :
     ForIn.forIn it init f = IterM.DefaultConsumers.forIn' (n := n)
-        (fun _ _ f x => monadLift x >>= f) γ it init _ (fun _ => id) (fun out _ acc => f out acc) := by
+        (fun _ _ f x => monadLift x >>= f) γ (fun _ _ _ => True) it init _ (fun _ => id)
+        (fun out _ acc => return ⟨← f out acc, trivial⟩) := by
   simp only [ForIn.forIn, forIn'_eq]
 
 @[congr] theorem IterM.forIn'_congr {α β : Type w} {m : Type w → Type w'}
@@ -189,23 +143,17 @@ theorem IterM.DefaultConsumers.forIn'_eq_forIn' {m : Type w → Type w'} {α : T
     {it : IterM (α := α) m β} {init : γ}
     {P : β → Prop} {hP : ∀ b, it.IsPlausibleIndirectOutput b → P b}
     {Q : β → Prop} {hQ : ∀ b, it.IsPlausibleIndirectOutput b → Q b}
-    {f : (b : β) → P b → (c : γ) → n (ForInStep γ)}
-    {g : (b : β) → Q b → (c : γ) → n (ForInStep γ)}
     (Pl : β → γ → ForInStep γ → Prop)
+    {f : (b : β) → P b → (c : γ) → n (Subtype (Pl b c))}
+    {g : (b : β) → Q b → (c : γ) → n (Subtype (Pl b c))}
     (wf : IteratorLoop.WellFounded α m Pl)
-    (f' : (b : β) → P b → (c : γ) → n (Subtype (Pl b c)))
-    (hf : ∀ b h c, f b h c = Subtype.val <$> f' b h c)
-    (g' : (b : β) → Q b → (c : γ) → n (Subtype (Pl b c)))
-    (hg : ∀ b h c, g b h c = Subtype.val <$> g' b h c)
-    (hfg : ∀ b c, (hPb : P b) → (hQb : Q b) → f' b hPb c = g' b hQb c) :
-    IterM.DefaultConsumers.forIn' lift γ it init P hP f =
-      IterM.DefaultConsumers.forIn' lift γ it init Q hQ g := by
-  rw [forIn'_eq_match_step Pl wf f' hf, forIn'_eq_match_step Pl wf g' hg]
+    (hfg : ∀ b c, (hPb : P b) → (hQb : Q b) → f b hPb c = g b hQb c) :
+    IterM.DefaultConsumers.forIn' lift γ Pl it init P hP f =
+      IterM.DefaultConsumers.forIn' lift γ Pl it init Q hQ g := by
+  rw [forIn'_eq_match_step Pl wf, forIn'_eq_match_step Pl wf]
   congr; ext step
   split
-  · rw [hf, hg]
-    simp only [map_eq_pure_bind, bind_assoc, pure_bind]
-    congr
+  · congr
     · apply hfg
     · ext forInStep
       match forInStep with
@@ -239,34 +187,19 @@ theorem IterM.forIn'_eq_match_step {α β : Type w} {m : Type w → Type w'} [It
   rw [IterM.forIn'_eq, DefaultConsumers.forIn'_eq_match_step]
   · apply bind_congr; intro step
     cases step.inflate using PlausibleIterStep.casesOn
-    · simp only
+    · simp only [bind_assoc]
       apply bind_congr
       intro forInStep
       cases forInStep
       · simp
-      · simp only [forIn'_eq] --[bind_pure_comp, pure_bind, forIn'_eq]
-        refine DefaultConsumers.forIn'_eq_forIn' (α := α) (m := m) (n := n) ?_ ?_ ?_ ?_ ?_ ?_ ?_
-        · exact fun _ _ _ => True
-        · exact IteratorLoop.wellFounded_of_finite
-        · exact fun out h c => (⟨·, trivial⟩) <$> f out h c
-        · simp
-        · exact fun out h c => (⟨·, trivial⟩) <$> f out (.indirect ⟨_, rfl, ‹_›⟩ h) c
-        · simp
-        · simp
+      · simp only [forIn'_eq, pure_bind]
+        exact DefaultConsumers.forIn'_eq_forIn' (α := α) (m := m) (n := n) _
+          IteratorLoop.wellFounded_of_finite (by simp)
     · simp only [forIn'_eq]
-      refine DefaultConsumers.forIn'_eq_forIn' (α := α) (m := m) (n := n) ?_ ?_ ?_ ?_ ?_ ?_ ?_
-      · exact fun _ _ _ => True
-      · exact IteratorLoop.wellFounded_of_finite
-      · exact fun out h c => (⟨·, trivial⟩) <$> f out h c
-      · simp
-      · exact fun out h c => (⟨·, trivial⟩) <$> f out (.indirect ⟨_, rfl, ‹_›⟩ h) c
-      · simp
-      · simp
+      exact DefaultConsumers.forIn'_eq_forIn' (α := α) (m := m) (n := n) _
+          IteratorLoop.wellFounded_of_finite (by simp)
     · simp
-  · exact fun _ _ _ => True
   · exact IteratorLoop.wellFounded_of_finite
-  · exact fun out h c => (⟨·, trivial⟩) <$> f out h c
-  · simp
 
 theorem IterM.forIn_eq_match_step {α β : Type w} {m : Type w → Type w'} [Iterator α m β]
     [Finite α m] {n : Type w → Type w''} [Monad m] [Monad n] [LawfulMonad n]
